closer

Std/Tactic/Omega/Shadows.lean
@@ -16,7 +16,10 @@ of `c * v = j` and for each previously considered lower bound `c * v - f > (c * 
 def greyShadows (v m : Int) : List (Int × Int) → Option Nat → Prop
   | [], _ => False
   | (f, c) :: bounds, none =>
-    greyShadows v m ((f, c) :: bounds) (some ((c * m - c - m)/m).natAbs)
+    if c = 1 then
+      greyShadows v m bounds none
+    else
+      greyShadows v m ((f, c) :: bounds) (some ((c * m - c - m)/m).toNat)
   | (f, c) :: bounds, some 0 =>
     c * v - f = 0 ∨ c * v - f > (c * m - c - m)/m ∧ greyShadows v m bounds none
   | (f, c) :: bounds, some (j + 1) =>
@@ -27,10 +30,67 @@ decreasing_by sorry
 def greyShadows' (v m : Int) (lowerBounds : List (Int × Int)) : Prop :=
     ∃ l, l ∈ lowerBounds ∧ ∃ j : Nat, j ≤ (l.2 * m - l.2 - m)/m ∧ l.2 * v - l.1 = j
 
-theorem greyShadows_iff (v m : Int) (lowerBounds : List (Int × Int)) (sat : ∀ l, l ∈ lowerBounds → l.1 ≤ l.2 * v) :
-    greyShadows v m lowerBounds none ↔ greyShadows' v m lowerBounds :=
-  -- We'll need more intermediate steps here!
-  sorry
+theorem greyShadows_iff_aux :
+    greyShadows v m ((f, c) :: lowerBounds) (some j) ↔
+      (∃ j' : Nat, j' ≤ j ∧ c * v - f = j') ∨
+        ((c * m - c - m) / m < c * v - f ∧ greyShadows v m lowerBounds none) := by
+  induction j with
+  | zero =>
+    simp [greyShadows]
+  | succ j ih =>
+    rw [greyShadows, ih]
+    have : ∀ a, a ≤ j + 1 ↔ a = j + 1 ∨ a ≤ j := by
+      intro a
+      constructor
+      · exact fun h => or_comm.mp (Nat.le_or_eq_of_le_succ h)
+      · rintro (h | h)
+        · exact Nat.le_of_eq h
+        · exact Nat.le_succ_of_le h
+    simp only [this]
+    simp [exists_eq_or_imp]
+    rw [or_assoc]
+
+-- These sorries are just arithmetic:
+theorem greyShadows_of (v m : Int)
+    (two_le_m : 2 ≤ m)
+    (lowerBounds : List (Int × Int))
+    (lowerBounds_pos : ∀ l, l ∈ lowerBounds → 0 < l.2)
+    (sat : ∀ l, l ∈ lowerBounds → l.1 ≤ l.2 * v) :
+      greyShadows' v m lowerBounds → greyShadows v m lowerBounds none := by
+  induction lowerBounds with
+  | nil => simp [greyShadows, greyShadows']
+  | cons p lowerBounds ih =>
+    rcases p with ⟨f, c⟩
+    rw [greyShadows, greyShadows_iff_aux]
+    split <;> rename_i hc
+    · subst hc
+      rw [greyShadows']
+      have w : ∀ j : Nat, j ≤ (m - 1 - m) / m ↔ False := sorry
+      simp only [w, List.mem_cons, exists_eq_or_imp, Int.one_mul, false_and, exists_const, false_or]
+      rw [← greyShadows']
+      apply ih
+      · exact fun p m => lowerBounds_pos p (List.mem_cons_of_mem _ m)
+      · exact fun p m => sat p (List.mem_cons_of_mem _ m)
+    · replace hc : 2 ≤ c := sorry
+      rw [greyShadows']
+      simp
+      rw [← greyShadows']
+      intro h
+      rcases h with ⟨j, le, eq⟩ | h
+      · left
+        refine ⟨j, ?_, eq⟩
+        · rw [← Int.ofNat_le]
+          rw [Int.toNat_of_nonneg]
+          exact le
+          sorry
+      · rw [Classical.or_iff_not_imp_left]
+        simp
+        intro h'
+        constructor
+        · sorry
+        · apply ih _ _ h
+          · exact fun p m => lowerBounds_pos p (List.mem_cons_of_mem _ m)
+          · exact fun p m => sat p (List.mem_cons_of_mem _ m)
 
 def darkShadow (v : Int) : List (Int × Int) → List (Int × Int) → Prop
   | [], _ => True
@@ -42,7 +102,10 @@ where
   | (f, c), (f', c') :: upperBounds =>
     c * f' - c' * f ≥ c * c' - c - c' + 1 ∧ go (f, c) upperBounds
 
-theorem darkShadow_of_cons_right (h : darkShadow v l (q :: u)) : darkShadow v l u := sorry
+theorem darkShadow_of_cons_right (h : darkShadow v l (q :: u)) : darkShadow v l u := by
+  induction l with
+  | nil => simp [darkShadow]
+  | cons p l ih => sorry
 
 theorem darkShadow_iff (v : Int) (lowerBounds upperBounds : List (Int × Int)) :
     darkShadow v lowerBounds upperBounds ↔
@@ -87,8 +150,14 @@ theorem darkShadow_iff (v : Int) (lowerBounds upperBounds : List (Int × Int)) :
         intro l u l_mem u_mem
         exact h l u (.inr l_mem) u_mem
 
-theorem shadows_sat (v m : Int) (lowerBounds upperBounds : List (Int × Int))
-    (lowerBounds_sat : ∀ l, l ∈ lowerBounds → l.1 ≤ l.2 * v) :
+instance : @Trans Int Int Int (· ≤ ·) (· ≤ ·) (· ≤ ·) := sorry
+
+-- The sorries here are all easy.
+theorem shadows_sat (v m : Int) (two_le_m : 2 ≤ m) (lowerBounds upperBounds : List (Int × Int))
+    (lowerBounds_pos : ∀ l, l ∈ lowerBounds → 0 < l.2)
+    (lowerBounds_sat : ∀ l, l ∈ lowerBounds → l.1 ≤ l.2 * v)
+    (upperBounds_sat : ∀ u, u ∈ upperBounds → u.2 * v ≤ u.1)
+    (mh : ∀ u, u ∈ upperBounds → u.2 ≤ m) :
     (darkShadow v lowerBounds upperBounds) ∨ (greyShadows v m lowerBounds none) := by
   rw [Classical.or_iff_not_imp_left]
   intro h
@@ -102,9 +171,21 @@ theorem shadows_sat (v m : Int) (lowerBounds upperBounds : List (Int × Int))
   rw [Classical.not_forall] at h
   obtain ⟨u_mem, h⟩ := h
   rw [Int.not_le] at h
-  rw [greyShadows_iff _ _ _ lowerBounds_sat, greyShadows']
+  apply greyShadows_of _ _ two_le_m _ lowerBounds_pos lowerBounds_sat
+  rw [greyShadows']
   refine ⟨l, l_mem, ?_⟩
-  refine ⟨(l.2 * v - l.1).natAbs, ?_⟩
+  rcases l with ⟨c, f⟩
+  rcases u with ⟨c', f'⟩
+  refine ⟨(f * v - c).natAbs, ?_⟩
+  specialize upperBounds_sat _ u_mem
+  specialize lowerBounds_sat _ l_mem
+  specialize mh _ u_mem
+  dsimp at *
   rw [Int.natAbs_of_nonneg sorry] -- easy from `lowerBounds_sat`
   refine ⟨?_, rfl⟩
-  sorry -- Still a bit of work from here, need a fact about `m`
+  have w := calc
+    f' * (f * v - c) = f * (f' * v) - f' * c := sorry
+    _ ≤ f * c' - f' * c := sorry
+    _ ≤ f * f' - f - f' := sorry
+  have w' : f * v - c ≤ (f * f' - f - f') / f' := sorry
+  sorry
